src/ReactorModel/Determinism/State.lean
@@ -14,8 +14,8 @@ theorem exec_objₘ_rcn_eq {s : State} (m₁ : rcn ∈ s.rtr[.rcn]) (m₂ : rcn 
     s.rtr⟦m₁⟧ = (s.exec rcn').rtr⟦m₂⟧ :=
   Equivalent.objₘ_rcn_eq (s.exec_equiv rcn') m₁ |>.choose_spec
 
-theorem target_not_mem_indep_output {s : State} {i} {rcn₁ rcn₂ : ID}
-    (hi : rcn₁ ≮[s.rtr] rcn₂) (m₂ : rcn₂ ∈ s.rtr[.rcn]) (hd : ⟨cpt, i⟩ ∈ s.rtr⟦m₂⟧.deps .in) : 
+theorem target_not_mem_indep_output {s : State} {i} {rcn₁ rcn₂ : ID} {m₂ : rcn₂ ∈ s.rtr[.rcn]}
+    (hi : rcn₁ ≮[s.rtr]≯ rcn₂) (hd : ⟨cpt, i⟩ ∈ s.rtr⟦m₂⟧.deps .in) : 
     (s.output rcn₁).All₂ (¬·.Targets cpt i) := by
   apply List.all₂_iff_forall.mpr
   intro c hc
@@ -23,35 +23,42 @@ theorem target_not_mem_indep_output {s : State} {i} {rcn₁ rcn₂ : ID}
   split at hc <;> try contradiction
   case inl m₁ =>
     cases cpt
-    case' prt, act => 
-      intro ⟨⟩ 
-      exact absurd hd $ hi.deps_disjoint m₁ m₂ (by simp) (s.rtr⟦m₁⟧.targetMemDeps hc)
-    case stv =>
-      sorry
-
-theorem exec_indep_restriction_eq {s : State} (hn : rcn₁ ≠ rcn₂) (hi : rcn₁ ≮[s.rtr] rcn₂) (m₁ m₂) : 
+    all_goals
+      intro ⟨⟩
+      apply absurd hd
+    case stv => exact hi.state_mem_rcn₁_deps_not_mem_rcn₂_deps m₂ hc
+    all_goals 
+      have h := s.rtr⟦m₁⟧.targetMemDeps hc
+      exact NotDependent.deps_disjoint hi.left h (by simp [Change.Normal.target]) m₂
+    
+theorem exec_indep_restriction_eq {s : State} (hi : rcn₁ ≮[s.rtr]≯ rcn₂) (m₁ m₂) : 
     input.restriction (s.exec rcn₁) rcn₂ m₂ cpt = input.restriction s rcn₂ m₁ cpt := by 
   simp [input.restriction]
   rw [←exec_objₘ_rcn_eq m₁ m₂]
   apply Partial.ext_restrict 
-  intro i hd
-  exact Reactor.apply'_preserves_unchanged $ target_not_mem_indep_output hi m₁ hd  
+  intro _ hd
+  exact Reactor.apply'_preserves_unchanged $ target_not_mem_indep_output hi hd  
   
-theorem exec_indep_input_eq {s : State} (hn : rcn₁ ≠ rcn₂) (hi : rcn₁ ≮[s.rtr] rcn₂) : 
-    (s.exec rcn₁).input rcn₂ = s.input rcn₂ := by 
+theorem exec_indep_input_eq {s : State} (hi : rcn₁ ≮[s.rtr]≯ rcn₂) (m₁ : rcn₂ ∈ s.rtr[.rcn]) 
+    (m₂ : rcn₂ ∈ (s.exec rcn₁).rtr[.rcn]) : (s.exec rcn₁).input rcn₂ = s.input rcn₂ := by 
   simp [input]
+  split <;> try contradiction
+  refine ⟨?_, by simp [exec]⟩
+  ext1
+  exact exec_indep_restriction_eq hi m₁ m₂
+    
+theorem exec_indep_output_eq {s : State} (hi : rcn₁ ≮[s.rtr]≯ rcn₂) : 
+    (s.exec rcn₁).output rcn₂ = s.output rcn₂ := by 
+  simp [output]
   split <;> split 
-  case inr.inr => simp [exec]
+  case inl.inl m₂ m₁ => simp [exec_indep_input_eq hi m₁ m₂, exec_objₘ_rcn_eq m₁ m₂]
+  case inr.inr => rfl
   case inr.inl h => 
     have := Equivalent.mem_iff (Equivalent.symm $ Reactor.apply'_equiv _ $ s.output rcn₁) |>.mp h
     contradiction
   case inl.inr h _ =>
     have := Equivalent.mem_iff (Reactor.apply'_equiv _ $ s.output rcn₁) |>.mp h
     contradiction
-  case inl.inl m₂ m₁ =>
-    refine ⟨?_, by simp [exec]⟩
-    ext1
-    exact exec_indep_restriction_eq hn hi m₁ m₂
-    
+
 namespace State
 namespace Execution
